Propagated evaluator changes to translation code.

lean/evaluator.lean
@@ -5,39 +5,99 @@ import tactic.find
 
 -- FIXME: move
 namespace mc_semantics
+
+-- This represents only nats (not lhs or expression binders), and is
+-- used to instantiate nat_exprs
+@[reducible]
+def nat_env := list (option nat)
+
 namespace nat_expr
 
--- def eval (e : environment) : nat_expr -> option ℕ 
---   | (nat_expr.lit n)     := some n
---   | (nat_expr.var idx)   := list.nth e idx >>= λa, a.as_nat
---   | (nat_expr.add e1 e2) := (+) <$> (eval e1) <*> (eval e2) 
---   | (nat_expr.sub e1 e2) := (λx y, x - y) <$> (eval e1) <*> (eval e2) 
---   | (nat_expr.mul e1 e2) := (*) <$> (eval e1) <*> (eval e2) 
---   | (nat_expr.div e1 e2) := (/) <$> (eval e1) <*> (eval e2) 
+@[reducible]
+def eval (e : nat_env) : nat_expr -> option ℕ 
+  | (lit n)     := some n
+  | (var idx)   := monad.join (list.nth e idx)
+  | (add e1 e2) := (+) <$> (eval e1) <*> (eval e2) 
+  | (sub e1 e2) := (λx y, x - y) <$> (eval e1) <*> (eval e2) 
+  | (mul e1 e2) := (*) <$> (eval e1) <*> (eval e2) 
+  | (div e1 e2) := (/) <$> (eval e1) <*> (eval e2) 
+
+def wf_nat_expr (nenv : nat_env) : nat_expr -> Prop 
+  | (lit _)     := true
+  | (var idx)   := option.is_some (monad.join (list.nth nenv idx))
+  | (add e1 e2) := wf_nat_expr e1 ∧ wf_nat_expr e2
+  | (sub e1 e2) := wf_nat_expr e1 ∧ wf_nat_expr e2
+  | (mul e1 e2) := wf_nat_expr e1 ∧ wf_nat_expr e2
+  | (div e1 e2) := wf_nat_expr e1 ∧ wf_nat_expr e2
+
+lemma eval_add_eq {e} {x y} : eval e (x + y) = (+) <$> (eval e x) <*> (eval e y) :=
+  by { cases x; cases y; simp [ has_add.add, nat_expr.do_add, nat_expr.eval] }
+
+lemma eval_sub_eq {e} {x y} : eval e (x - y) = (λx y, x - y) <$> (eval e x) <*> (eval e y) :=
+  by { cases x; cases y; simp [ has_sub.sub, nat_expr.do_sub, nat_expr.eval]  }
+
+lemma eval_mul_eq {e} {x y} : eval e (x * y) = (*) <$> (eval e x) <*> (eval e y) :=
+  by { cases x; cases y; simp [ has_mul.mul, nat_expr.do_mul, nat_expr.eval] }
 
 @[reducible]
-def eval : nat_expr -> ℕ 
-  | (nat_expr.lit n)     := n
-  -- | (nat_expr.var idx)   := match list.nth nat_env idx with | (some (some n)) := n | _ := 0 end
-  | (nat_expr.var idx)   := 0
- -- FIXME, maybe use sorry?
-  | (nat_expr.add e1 e2) := (eval e1) + (eval e2) 
-  | (nat_expr.sub e1 e2) := (eval e1) - (eval e2) 
-  | (nat_expr.mul e1 e2) := (eval e1) * (eval e2) 
-  | (nat_expr.div e1 e2) := (eval e1) / (eval e2) 
+def eval_default (e : nat_env) : nat_expr -> ℕ 
+  | (lit n)     := n
+  | (var idx)   := match list.nth e idx with | (some (some n)) := n | _ := 0 end
+  | (add e1 e2) := (eval_default e1) + (eval_default e2) 
+  | (sub e1 e2) := (eval_default e1) - (eval_default e2) 
+  | (mul e1 e2) := (eval_default e1) * (eval_default e2) 
+  | (div e1 e2) := (eval_default e1) / (eval_default e2) 
+
+-- instance {nenv} : decidable_pred (wf_nat_expr nenv) := 
+-- begin
+--   unfold decidable_pred,
+--   intros e,
+--   induction e; simp [wf_nat_expr],
+--   case lit { apply is_true, trivial },
+--   case var { apply coe_decidable_eq },
+--   apply_instance, 
+  
+-- end
+
+lemma eval_default_add_eq {e} {x y} : eval_default e (x + y) = (eval_default e x) + (eval_default e y) :=
+  by { cases x; cases y; simp [ has_add.add, nat_expr.do_add, eval_default] }
+
+lemma eval_default_sub_eq {e} {x y} : eval_default e (x - y) = (eval_default e x) - (eval_default e y) :=
+  by { cases x; cases y; simp [ has_sub.sub, nat_expr.do_sub, nat_expr.eval_default]  }
+
+lemma eval_default_mul_eq {e} {x y} : eval_default e (x * y) = (eval_default e x) * (eval_default e y) :=
+  by { cases x; cases y; simp [ has_mul.mul, nat_expr.do_mul, nat_expr.eval_default] }
+
+
+-- @[reducible]
+-- def eval : nat_expr -> ℕ 
+--   | (nat_expr.lit n)     := n
+--   -- | (nat_expr.var idx)   := match list.nth nat_env idx with | (some (some n)) := n | _ := 0 end
+--   | (nat_expr.var idx)   := 0
+--  -- FIXME, maybe use sorry?
+--   | (nat_expr.add e1 e2) := (eval e1) + (eval e2) 
+--   | (nat_expr.sub e1 e2) := (eval e1) - (eval e2) 
+--   | (nat_expr.mul e1 e2) := (eval e1) * (eval e2) 
+--   | (nat_expr.div e1 e2) := (eval e1) / (eval e2) 
 
 end nat_expr
 
 namespace type 
 
 @[reducible]
-def eval : type -> type 
-  | (bv e) := bv e.eval
-  | (fn arg res) := fn (eval arg) (eval res)
-  | tp     := tp
+def eval (nenv : nat_env) : type -> option type 
+  | (bv e) := (λn, bv (nat_expr.lit n)) <$> nat_expr.eval nenv e
+  | (fn arg res) := fn <$> (eval arg) <*> (eval res)
+  | tp     := return tp
+
+def eval_default (nenv : nat_env) : type -> type 
+  | (bv e) := bv (nat_expr.lit (nat_expr.eval_default nenv e))
+  | (fn arg res) := fn (eval_default arg) (eval_default res)
+  | tp           := tp
 
 end type
 end mc_semantics
+
 
 namespace x86
 
@@ -46,6 +106,19 @@ open mc_semantics.type
 
 @[reducible]
 def machine_word := bitvec 64
+
+namespace reg
+
+def inject : Π(rtp : gpreg_type), bitvec rtp.width -> machine_word -> machine_word
+  | gpreg_type.reg32 b _   := bitvec.append (bitvec.zero 32) b
+  | gpreg_type.reg8h b old := old.set_bits 48 b (of_as_true trivial)
+  | rtp              b old := old.set_bits (64 - rtp.width) b (begin cases rtp; dec_trivial_tac end)
+
+def project : Π(rtp : gpreg_type), machine_word -> bitvec rtp.width
+  | gpreg_type.reg8h b := b.get_bits 48 8 (by dec_trivial_tac)
+  | rtp              b := b.get_bits (64 - rtp.width) rtp.width (begin cases rtp; dec_trivial_tac end)
+
+end reg
 
 def memory := rbmap machine_word (bitvec 8) (bitvec.ult) -- FIXME: 8?
 
@@ -148,28 +221,8 @@ end machine_state
 --   | bit : bool -> value bit
 --   | func  {tp tp' : type} : (value tp -> value tp') -> value (fn tp tp')
 
-@[reducible]
-def value : type -> Type
-  | (bv e) := bitvec e.eval -- We use the _normalised_ value here.
-  | bit    := bool
-  | float  := unit -- FIXME
-  | double := unit -- FIXME
-  | x86_80 := unit -- FIXME  
-  | (fn arg res) := (value arg) -> (value res)
-
-namespace value
-
-def repr : Π{tp : type}, value tp -> string
-  | (bv e) b                := has_repr.repr b
-  | (fn _ _ ) _             := "<function>"
-  | _ _                     := "Unsupported type"
-
-instance value_repr {tp : type} : has_repr (value tp) := ⟨repr⟩
-
-end value
-
-inductive arg_lval 
-  | reg {tp : type} : reg tp -> arg_lval
+inductive arg_lval
+  | reg {} {tp : type} : reg tp -> arg_lval
   | memloc (width : ℕ) (addr : machine_word) : arg_lval
 
 namespace arg_lval
@@ -182,20 +235,59 @@ instance arg_lval_repr : has_repr arg_lval := ⟨repr⟩
 
 end arg_lval
 
+section with_nat_env
+
+parameter (nenv : nat_env)
+
+@[reducible]
+def eval_nat_expr (e : nat_expr) : nat
+  := nat_expr.eval_default nenv e
+
+@[reducible]
+def eval_type : type -> type := type.eval_default nenv
+  -- | (bv e) := bv (nat_expr.lit (eval_nat_expr e))
+  -- | (fn arg res) := fn (eval_type arg) (eval_type res)
+  -- | tp     := tp
+
+@[reducible]
+def value : type -> Type
+  | (bv e) := bitvec (eval_nat_expr e) -- We use the _normalised_ value here.
+  | bit    := bool
+  | float  := unit -- FIXME
+  | double := unit -- FIXME
+  | x86_80 := unit -- FIXME  
+  | (fn arg res) := (value arg) -> (value res)
+
+-- namespace value
+
+-- def value.repr : Π{tp : type}, value tp -> string
+--   | (bv e) b                := has_repr.repr b
+--   | (fn _ _ ) _             := "<function>"
+--   | _ _                     := "Unsupported type"
+
+
+-- instance value_repr {tp : type} : has_repr (value tp) := ⟨value.repr⟩
+
+-- end value
+
 -- Corresponding to the binder type, more or less.
 inductive arg_value 
+  -- natv is here for completeness --- the presumption is that a
+  -- one_of param is only used in types, but in case it is not, we
+  -- include a binding in the environment,
+  | natv             : ℕ        -> arg_value 
   | lval             : arg_lval -> arg_value
   | rval {tp : type} : value tp -> arg_value
 
-namespace arg_value
+-- namespace arg_value
 
-def repr : arg_value -> string 
-  | (lval l) := l.repr
-  | (rval v)  := v.repr
+-- def repr : arg_value -> string 
+--   | (lval l) := l.repr
+--   | (rval v)  := v.repr
 
-instance arg_value_repr : has_repr arg_value := ⟨repr⟩
+-- instance arg_value_repr : has_repr arg_value := ⟨repr⟩
 
-end arg_value
+-- end arg_value
 
 @[reducible]
 def environment := list arg_value
@@ -205,19 +297,20 @@ structure evaluator_state : Type :=
   (environment : environment) -- read only, but reading can fail
   (locals : rbmap ℕ (sigma value))
 
-namespace evaluator_state
+-- namespace evaluator_state
 
-def empty : evaluator_state := 
+def evaluator_state.empty : evaluator_state := 
   { machine_state := machine_state.empty
   , environment   := []
   , locals        := mk_rbmap ℕ (sigma value)
   }
 
-end evaluator_state
+-- end evaluator_state
 
 -- Monad for evaluating with failure.  This nesting might be useful to get the ip where things break?
 @[reducible]
 def evaluator := state_t evaluator_state (except string)
+
 
 -- FIXME: are these an oversight in the stdlib? 
 instance (ε): monad_except ε (except ε) := 
@@ -229,7 +322,7 @@ instance (ε) (m) [monad_except ε m] : has_orelse m :=
 instance (ε) [inhabited ε] : alternative (except ε) := 
   { failure := λα, except.error (default ε)}
 
-namespace type
+-- namespace type
 
 -- If evaluation of the expr fails, we return the original type.  
 -- def normalise (e : environment) : type -> type
@@ -242,47 +335,49 @@ namespace type
 -- instance (e) : decidable_rel (equiv e) :=
 --   λa b, begin simp [equiv], apply_instance end
 
-end type
+-- end type
 
-namespace value
+-- namespace value
 
-lemma type_eval_is_id: Π{tp : type}, value tp.eval = value tp :=
+lemma value.type_eval_is_id: Π{tp : type}, value (eval_type tp) = value tp :=
 begin  
   intros,
   induction tp,
   case bv { refl },
-  case fn { simp [value], rw [ tp_ih_arg, tp_ih_res ] },
+  case fn { simp [value, eval_type, type.eval_default], rw [ tp_ih_arg, tp_ih_res ] },
   repeat { refl }
 end
 
-def eval_cong {tp tp' : type} (pf : tp.eval = tp'.eval) (v : value tp) : value tp' :=
+def value.eval_cong {tp tp' : type} (pf : eval_type tp = eval_type tp') (v : value tp) : value tp' :=
 begin
-  rw <- type_eval_is_id,
-  rw <- type_eval_is_id at v,
+  rw <- value.type_eval_is_id,
+  rw <- value.type_eval_is_id at v,
   exact (eq.rec v pf)   
 end
 
 -- This allows us to resolve arith in nat_exprs
-def type_check {tp : type} (v : value tp) (tp' : type) : evaluator (value tp') :=
-  if H : tp.eval = tp'.eval
-  then return (eval_cong H v)
+def value.type_check {m} [monad m] [monad_except string m] (tp : type) (v : value tp) (tp' : type) 
+  : m (value tp') :=
+  if H : eval_type tp = eval_type tp'
+  then return (value.eval_cong H v)
   else throw "type_check: arg type mismatch"
 
-end value
+-- end value
 
-namespace evaluator
 
-def run {a : Type} (m : evaluator a) (s : evaluator_state) : except string (a × evaluator_state) :=
+-- namespace evaluator
+
+def evaluator.run {a : Type} (m : evaluator a) (s : evaluator_state) : except string (a × evaluator_state) :=
   (m.run s)
 
-def read_memory_at (addr : machine_word) (n : ℕ) : evaluator (bitvec (8 * n)) := do
+def evaluator.read_memory_at (addr : machine_word) (n : ℕ) : evaluator (bitvec (8 * n)) := do
     s <- get, 
     match s.machine_state.read_word addr n with
     | none := throw "read_memory_at: no bytes at addr" 
     | (some w) := return w
     end
 
-def arg_at_idx (idx : ℕ) : evaluator arg_value :=
+def evaluator.arg_at_idx (idx : ℕ) : evaluator arg_value :=
   do s <- get,
      match s.environment.nth idx with
        | (some a) := return a
@@ -291,80 +386,52 @@ def arg_at_idx (idx : ℕ) : evaluator arg_value :=
 
 -- We should factor out the type check, although it might depend on
 -- the functor (value in this case) if we generalise equality
-def local_at_idx (idx : ℕ) (tp : type) : evaluator (value tp) :=
+def evaluator.local_at_idx (idx : ℕ) (tp : type) : evaluator (value tp) :=
   do s <- get,
      match s.locals.find idx with
-     | (some (sigma.mk tp' v)) := v.type_check tp
+     | (some (sigma.mk tp' v)) := value.type_check _ v tp
      | none     := throw "local_at_idx: no arg at idx"
      end
-
--- def normalise_type (t : type) : evaluator type :=
---   do s <- get,
---      return (type.normalise s.environment t)
-def with_nat_expr_as_nat {a} : Π(e : nat_expr), (Πn, e = nat_expr.lit n -> evaluator a) -> evaluator a
- | (nat_expr.lit n) f := f n rfl
- | _ _ := throw "type_as_bv: Not a lit BV"
-
-def with_nat_expr_as_nat' (f : nat_expr -> Type) 
-  : Π(e : nat_expr), (Πn, evaluator (f (nat_expr.lit n))) -> evaluator (f e)
- | (nat_expr.lit n) m := m n
- | _ _ := throw "type_as_bv: Not a lit BV"
-
-def with_type_as_bv {a} : Π(tp : type), (Πn, tp = bv (nat_expr.lit n) -> evaluator a) -> evaluator a
- | (bv (nat_expr.lit n)) f := f n rfl
- | _ _ := throw "type_as_bv: Not a lit BV"
-
-end evaluator
-
   
-namespace reg
-
-def inject : Π(rtp : gpreg_type), bitvec rtp.width -> machine_word -> machine_word
-  | gpreg_type.reg32 b _   := bitvec.append (bitvec.zero 32) b
-  | gpreg_type.reg8h b old := old.set_bits 48 b (of_as_true trivial)
-  | rtp              b old := old.set_bits (64 - rtp.width) b (begin cases rtp; dec_trivial_tac end)
-
-def project : Π(rtp : gpreg_type), machine_word -> bitvec rtp.width
-  | gpreg_type.reg8h b := b.get_bits 48 8 (by dec_trivial_tac)
-  | rtp              b := b.get_bits (64 - rtp.width) rtp.width (begin cases rtp; dec_trivial_tac end)
-
-def set : Π{tp : type}, reg tp -> value tp -> evaluator unit
-  | ._ (concrete_gpreg idx rtp) b := 
-    modify (λ(s : evaluator_state), { s with machine_state := machine_state.update_gpreg idx (inject rtp b) s.machine_state })
-  | ._ (concrete_flagreg idx)   b := 
+def reg.set : Π{tp : type}, reg tp -> value tp -> evaluator unit
+  | ._ (reg.concrete_gpreg idx rtp) b := 
+    modify (λ(s : evaluator_state), { s with machine_state := machine_state.update_gpreg idx (reg.inject rtp b) s.machine_state })
+  | ._ (reg.concrete_flagreg idx)   b := 
     modify (λ(s : evaluator_state), { s with machine_state := machine_state.update_flag idx (λ_, b) s.machine_state })
 
-def read : Π{tp : type}, reg tp -> evaluator (value tp)
-  | ._ (concrete_gpreg idx rtp) := do s <- get,
-                                      return (project rtp (s.machine_state.get_gpreg idx))
-  | ._ (concrete_flagreg idx)   := do s <- get,
-                                      return (s.machine_state.get_flag idx)
+def reg.from_state : Π{tp : type}, reg tp -> machine_state -> value tp
+  | ._ (reg.concrete_gpreg idx rtp) s := reg.project rtp (s.get_gpreg idx)
+  | ._ (reg.concrete_flagreg idx)   s := s.get_flag idx
 
-end reg
+def reg.read {tp : type} (r : reg tp) : evaluator (value tp) := do s <- get, return (reg.from_state r s.machine_state)
 
-namespace arg_lval 
+-- namespace arg_lval 
 
-def to_value : arg_lval -> Π(tp : type), evaluator (value tp)
-  | (@reg tp r) tp' := 
-    if H : tp = tp'
-    then eq.rec r.read H
-    else throw "to_value: reg type mismatch"
-  | (memloc width addr) tp' := do
+def arg_lval.to_value' {m} [monad m] [monad_except string m] 
+  (s : machine_state)
+  : arg_lval -> Π(tp : type), m (value tp)
+  | (@arg_lval.reg tp r) tp' := value.type_check tp (reg.from_state r s) tp'
+  | (arg_lval.memloc width addr) tp' :=
+    match s.read_word addr (width / 8) with
+    | none := throw "arg_lval.to_value': no bytes at addr" 
+    | (some w) := value.type_check (bv (8 * (width / 8))) w tp'
+    end
+
+def arg_lval.to_value : arg_lval -> Π(tp : type), evaluator (value tp)
+  | (@arg_lval.reg tp r) tp' := do v <- reg.read r,
+                                   value.type_check tp v tp'
+  | (arg_lval.memloc width addr) tp' := do
     v <- evaluator.read_memory_at addr (width / 8),
-    @value.type_check (bv (8 * (width / 8))) v tp'
+    value.type_check (bv (8 * (width / 8))) v tp'
 
-def set_value : arg_lval -> Π{tp : type}, value tp -> evaluator unit
-  | (@reg tp r) tp' v := do v' <- value.type_check v tp,
-                            r.set v'
-  | (memloc width addr) (bv (nat_expr.lit n)) bytes :=  -- FIXME: use nat_expr.eval instead of assuming lit
+def arg_lval.set_value : arg_lval -> Π{tp : type}, value tp -> evaluator unit
+  | (@arg_lval.reg tp r) tp' v := do v' <- value.type_check _ v tp,
+                                     reg.set r v'
+  | (arg_lval.memloc width addr) (bv (nat_expr.lit n)) bytes :=  -- FIXME: use nat_expr.eval instead of assuming lit
     if H : n = 8 * (width / 8)
     then modify (λs, { s with machine_state := s.machine_state.store_word addr (bitvec.cong H bytes) })
     else throw "arg_lval.set_value: width mismatch"
   | _ _ _ := throw "arg_lval.set_value: malformed set"
-
-end arg_lval 
-
-namespace arg_value
 
 -- def read_memory_at (av : arg_value) (n : ℕ) : evaluator (bitvec (8 * n)) :=
 --   match av with 
@@ -373,47 +440,41 @@ namespace arg_value
 --   end
 
 -- Can fail if types mismatch
-def to_value : arg_value -> Π(tp : type), evaluator (value tp)
-  | (lval l) tp := l.to_value tp
-  | (rval v) tp := v.type_check tp
+def arg_value.to_value : arg_value -> Π(tp : type), evaluator (value tp)
+  | (arg_value.natv _ _)  _ := throw "arg_value.to_value: saw a natv"
+  | (arg_value.lval _ l) tp := arg_lval.to_value l tp
+  | (arg_value.rval v) tp := value.type_check _ v tp
 
-def set_value : arg_value -> Π{tp : type}, value tp -> evaluator unit
-  | (lval l) tp v := l.set_value v
+def arg_value.set_value : arg_value -> Π{tp : type}, value tp -> evaluator unit
+  | (arg_value.lval _ l) tp v := arg_lval.set_value l v
   | _ _ _ := throw "arg_value.set_value: not an lvalue"
 
-end arg_value
-
-namespace addr
-
-def read : Π{n : ℕ}, addr n -> evaluator (value (bv (8 * n)))
+def addr.read : Π{n : ℕ}, addr n -> evaluator (value (bv (8 * n)))
   | n (addr.arg idx) := do 
       av <- evaluator.arg_at_idx idx,
-      av.to_value (bv (8 * n)) -- FIXME: we should really check if this is a memloc first.
+      arg_value.to_value av (bv (8 * n)) -- FIXME: we should really check if this is a memloc first.
       -- w  <- av.read_memory_at n,
       -- return (value.bv w)
 
-def set : Π{n : ℕ}, addr n -> value (bv (8 * n)) -> evaluator unit
+def addr.set : Π{n : ℕ}, addr n -> value (bv (8 * n)) -> evaluator unit
   | n (addr.arg idx) v := do 
       av <- evaluator.arg_at_idx idx, -- FIXME: we should really check if this is a memloc first.
-      av.set_value v
+      arg_value.set_value av v
     
-end addr
+def lhs.set : Π{tp : type}, lhs tp -> value tp -> evaluator unit
+  | ._ (lhs.reg r) v      := reg.set r v
+  | ._ (lhs.addr a) v     := addr.set a v
+  | ._ (lhs.arg idx _tp) v := do av <- evaluator.arg_at_idx idx,
+                                 -- fixme: we ignore tp here?
+                                 arg_value.set_value av v
+  | ._ (lhs.streg idx) v  := throw "lhs.set: unsupported FP write"
 
-namespace lhs
-
-def set : Π{tp : type}, lhs tp -> value tp -> evaluator unit
-  | ._ (reg r) v      := r.set v
-  | ._ (addr a) v     := a.set v
-  | ._ (arg idx _tp) v := do av <- evaluator.arg_at_idx idx, av.set_value v -- fixme: we ignore tp here?
-  | ._ (streg idx) v  := throw "lhs.set: unsupported FP write"
-
-def read : Π{tp : type}, lhs tp -> evaluator (value tp)
-  | ._ (reg r)       := r.read
-  | ._ (addr a)      := a.read
-  | ._ (arg idx tp)  := do av <- evaluator.arg_at_idx idx, av.to_value tp
-  | ._ (streg idx)   := throw "lhs.read: unsupported FP read"
-
-end lhs
+def lhs.read : Π{tp : type}, lhs tp -> evaluator (value tp)
+  | ._ (lhs.reg r)       := reg.read r
+  | ._ (lhs.addr a)      := addr.read a
+  | ._ (lhs.arg idx tp)  := do av <- evaluator.arg_at_idx idx, 
+                                  arg_value.to_value av tp
+  | ._ (lhs.streg idx)   := throw "lhs.read: unsupported FP read"
 
 -- This is the least-worst option.  The other alternative is to have a
 -- value constructor for functions, which we only need here.
@@ -431,24 +492,21 @@ inductive {u v} hlist {α : Type u} (f : α -> Type v): list α -> Type (max u v
 --   end
 -- end nat_expr
 
-namespace prim
- 
 section
 
 local infixr `.→`:30 := fn
 
-def prim_binop (e : nat_expr) (p : Π{n : ℕ}, bitvec n -> bitvec n -> bitvec n) :=
-  evaluator.with_nat_expr_as_nat' (λi, value (bv i .→ bv i .→ bv i)) e (λn, return (@p n))
+-- def prim_binop (e : nat_expr) (p : Π{n : ℕ}, bitvec n -> bitvec n -> bitvec n) :=
+--   evaluator.with_nat_expr_as_nat' (λi, value (bv i .→ bv i .→ bv i)) e (λn, return (@p n))
 
-lemma eval_add_eq {x y} : nat_expr.eval (x + y) =  (x.eval + y.eval) :=
-  by { cases x; cases y; simp [has_add.add, nat_expr.do_add, nat_expr.eval] }
+-- lemma eval_add_eq {x y} : eval_nat_expr (x + y) =  (eval_nat_expr x + eval_nat_expr y) :=
+-- begin
+--   simp [eval_nat_expr, nat_expr.eval_add_eq, has_seq.seq], 
+-- end
 
-lemma eval_sub_eq {x y} : nat_expr.eval (x - y) = (x.eval - y.eval) :=
-  by { cases x; cases y; simp [ has_sub.sub, nat_expr.do_sub, nat_expr.eval]}
-
-lemma eval_mul_eq {x y} : nat_expr.eval (x * y) = (x.eval * y.eval) :=
-  by { cases x; cases y; simp [ has_mul.mul, nat_expr.do_mul, nat_expr.eval]}
-
+  -- by { cases x; cases y; simp [
+  --                              has_add.add, has_seq.seq, nat_expr.do_add
+  --                             , nat_expr.eval] }
 
 -- FIXME: move
 -- Might be easier to define in terms of to_int/from_int etc.
@@ -464,15 +522,18 @@ def bitvec.trunc {n} (m : ℕ) (p: m ≤ n) (x:bitvec n) : bitvec m :=
 def bit_to_bitvec (n : ℕ) (b : bool) : bitvec n := 
   if b then 1 else 0
 
-lemma eval_2: nat_expr.eval 2 = 2 := rfl
 
-def eval : Π{tp : type}, prim tp -> evaluator (value tp)
+lemma eval_default_2 {e} : nat_expr.eval_default e 2 = 2 := rfl
+
+lemma nat_expr_eval_2 : eval_nat_expr 2 = 2 := rfl
+
+def prim.eval : Π{tp : type}, prim tp -> evaluator (value tp)
   -- `(add i)` returns the sum of two i-bit numbers.
-  | ._ (add i)        := return bitvec.add
+  | ._ (prim.add i)        := return bitvec.add
   -- `(adc i)` returns the sum of two i-bit numbers and a carry bit.
-  | ._ (adc i)         := return (λx y b, bitvec.add x (bitvec.add y (bit_to_bitvec _ b)))
+  | ._ (prim.adc i)         := return (λx y b, bitvec.add x (bitvec.add y (bit_to_bitvec _ b)))
   -- `(mul i)` returns the product of two i-bit numbers.
-  | ._ (mul i)            := return bitvec.mul
+  | ._ (prim.mul i)            := return bitvec.mul
   -- `(quot i)` returns the quotient of two i-bit numbers.
   -- | quot (i:ℕ) : prim (bv i .→ bv i .→ bv i)
   -- `(rem i)` returns the remainder of two i-bit numbers.
@@ -484,24 +545,26 @@ def eval : Π{tp : type}, prim tp -> evaluator (value tp)
   -- `(slice w u l)` takes bits `u` through `l` out of a `w`-bit number.
   --  prim (bv w .→ bv (u+1-l))
   --  slice {w: ℕ} (u l k:ℕ) (H: w = k + (u + 1 - l)) (x: bitvec w) : bitvec (u + 1 - l)
-  | tp (slice w u l) := do
-       let n := u.eval + 1 - l.eval,
-       H <- assert (w.eval = (w.eval - n + n)),
+  | tp (prim.slice w u l) := do
+       let n := eval_nat_expr u + 1 - eval_nat_expr l,
+       H <- assert (eval_nat_expr w = (eval_nat_expr w - n + n)),
        return (begin
-         have rewr : value (bv (u + 1 - l)) = value (bv (nat_expr.lit n)) :=
-           begin simp [n, value, eval_sub_eq, eval_add_eq, nat_expr.eval], refl end,
+         have rewr : value nenv (bv (u + 1 - l)) = value nenv (bv (nat_expr.lit n)) :=
+           begin simp [n, value, nat_expr.eval_default_sub_eq
+                      , nat_expr.eval_default_add_eq
+                      , eval_nat_expr, nat_expr.eval_default], rw add_comm, refl end,
          simp [value], rw rewr,
-         exact (bitvec.slice u.eval l.eval (w.eval - (u.eval + 1 - l.eval)) H.default)
+         exact (bitvec.slice (eval_nat_expr nenv u) (eval_nat_expr nenv l) (eval_nat_expr nenv w - n) H.default)
         end)
   -- `(sext i o)` sign extends an `i`-bit number to a `o`-bit number.
-  | ._ (sext i o) := do H <- assert (i.eval ≤ o.eval),
-                        return (bitvec.sext o.eval H.default)
+  | ._ (prim.sext i o) := do H <- assert (eval_nat_expr i ≤ eval_nat_expr o),
+                             return (bitvec.sext (eval_nat_expr o) H.default)
   -- `(uext i o)` unsigned extension of an `i`-bit number to a `o`-bit number.
-  | ._ (uext i o) := do H <- assert (i.eval ≤ o.eval),
-                        return (bitvec.uext o.eval H.default)
+  | ._ (prim.uext i o) := do H <- assert (eval_nat_expr i ≤ eval_nat_expr o),
+                             return (bitvec.uext (eval_nat_expr o) H.default)
   -- `(trunc i o)` truncates an `i`-bit number to a `o`-bit number.
-  | ._ (trunc i o) := do H <- assert (o.eval ≤ i.eval),
-                         return (bitvec.trunc o.eval H.default)
+  | ._ (prim.trunc i o) := do H <- assert (eval_nat_expr o ≤ eval_nat_expr i),
+                              return (bitvec.trunc (eval_nat_expr o) H.default)
 
   -- `(bsf i)` returns the index of least-significant bit that is 1.
   -- | bsf   (i:ℕ) : prim (bv i .→ bv i)
@@ -510,15 +573,15 @@ def eval : Π{tp : type}, prim tp -> evaluator (value tp)
   -- `(bswap i)` reverses the bytes in the bitvector.
   -- | bswap (i:ℕ) : prim (bv i .→ bv i)
   -- `zero` is the zero bit
-  | ._ zero := return ff
+  | ._ prim.zero := return ff
   -- `one` is the one bit
-  | ._ one := return tt
+  | ._ prim.one := return tt
   -- `(eq tp)` returns `true` if two values are equal.
   -- | (eq (tp:type) : prim (tp .→ tp .→ bit)
   -- `(neq tp)` returns `true` if two values are not equal.
   -- | neq (tp:type) : prim (tp .→ tp .→ bit)
   -- `(neg tp)` Two's Complement negation.
-  | ._ (neg i) := return bitvec.neg
+  | ._ (prim.neg i) := return bitvec.neg
   -- `x87_fadd` adds two extended precision values using the flags in the x87 register.
   -- | x87_fadd : prim (x86_80 .→ x86_80 .→ x86_80)
   -- `float_to_x86_80` converts a float to an extended precision number (lossless)
@@ -528,34 +591,36 @@ def eval : Π{tp : type}, prim tp -> evaluator (value tp)
   -- `bv_to_x86_80` converts a bitvector to an extended precision number (lossless)
   -- | bv_to_x86_80  (w : one_of [16,32]) : prim (bv w .→ x86_80)
   -- `bvnat` constructs a bit vector from a natural number.
-  | ._ (bvnat w n) := return (bitvec.of_nat w.eval n.eval)
+  | ._ (prim.bvnat w n) := return (bitvec.of_nat (eval_nat_expr w) (eval_nat_expr n))
   -- `(bvadd i)` adds two i-bit bitvectors.
-  | ._ (bvadd i) := return bitvec.add
+  | ._ (prim.bvadd i) := return bitvec.add
   -- `(bvsub i)` substracts two i-bit bitvectors.
-  | ._ (bvsub i) := return bitvec.sub
+  | ._ (prim.bvsub i) := return bitvec.sub
   -- `(ssbb_overflows i)` true if signed sub overflows, the bit
   -- is a borrow bit.
   -- FIXME: is this correct?
-  | ._ (ssbb_overflows i) := return (λx y b, bitvec.slt x (x - y - bit_to_bitvec i.eval b))
+  | ._ (prim.ssbb_overflows i) := 
+    return (λx y b, bitvec.slt x (x - y - bit_to_bitvec (eval_nat_expr i) b))
   -- `(usbb_overflows i)` true if unsigned sub overflows,
   -- the bit is a borrow bit.
-  | ._ (usbb_overflows i) := return (λx y b, bitvec.ult x (x - y - bit_to_bitvec i.eval b))
+  | ._ (prim.usbb_overflows i) := return (λx y b, bitvec.ult x (x - y - bit_to_bitvec (eval_nat_expr i) b))
 
-  | ._ (uadc_overflows i) := return (λx y b, bitvec.ult (x + y + bit_to_bitvec i.eval b) x)
-  | ._ (sadc_overflows i) := return (λx y b, bitvec.slt (x + y + bit_to_bitvec i.eval b) x)
-  | ._ (and i) := return bitvec.and
-  | ._ (or i)  := return bitvec.or
-  | ._ (xor i) := return bitvec.xor
-  | ._ (shl i) := return (λx (y : bitvec i.eval), bitvec.shl x y.to_nat)
+  | ._ (prim.uadc_overflows i) := return (λx y b, bitvec.ult (x + y + bit_to_bitvec (eval_nat_expr i) b) x)
+  | ._ (prim.sadc_overflows i) := return (λx y b, bitvec.slt (x + y + bit_to_bitvec (eval_nat_expr i) b) x)
+  | ._ (prim.and i) := return bitvec.and
+  | ._ (prim.or i)  := return bitvec.or
+  | ._ (prim.xor i) := return bitvec.xor
+  | ._ (prim.shl i) := return (λx (y : bitvec (eval_nat_expr i)), bitvec.shl x y.to_nat)
   -- `(bvbit i)` interprets the second argument as a bit index and returns
   -- that bit from the first argument.
-  | ._ (bvbit i) := return (λx (y : bitvec i.eval), bitvec.nth x y.to_nat)
-  | ._ (complement i) := return bitvec.not
-  | ._ (bvcat i) := return (λx y, bitvec.cong
-                                    (by simp [eval_mul_eq, nat_expr.eval, eval_2, two_mul])
+  | ._ (prim.bvbit i) := return (λx (y : bitvec (eval_nat_expr i)), bitvec.nth x y.to_nat)
+  | ._ (prim.complement i) := return bitvec.not
+  | ._ (prim.bvcat i) := return (λx y, bitvec.cong
+                                    (begin simp [eval_nat_expr, nat_expr.eval_default_mul_eq, nat_expr.eval, eval_default_2, two_mul], 
+                                     end)
                                     (bitvec.append x y))
 -- | bv_least_nibble (i:ℕ) : prim (bv i .→ bv 4)
-  | ._ (msb i) := return bitvec.msb
+  | ._ (prim.msb i) := return bitvec.msb
 -- | least_byte (i:ℕ) : prim (bv i .→ bv 8)
 -- | even_parity (i:ℕ) : prim (bv i .→ bit)
   | _  _             := throw "prim.eval: unimplemented prim"
@@ -563,42 +628,30 @@ def eval : Π{tp : type}, prim tp -> evaluator (value tp)
 
 end
 
-end prim
-
-namespace expression
-
-def eval : Π{tp : type}, expression tp -> evaluator (value tp)
-  | ._ (primitive p) := p.eval
-  | ._ (app f a) := f.eval <*> a.eval
-  | ._ (get l)   := l.read
+def expression.eval : Π{tp : type}, expression tp -> evaluator (value tp)
+  | ._ (expression.primitive p) := prim.eval p
+  | ._ (expression.app f a) := (expression.eval f) <*> (expression.eval a)
+  | ._ (expression.get l)   := lhs.read l
   -- Return the expression in the local variable at the given index.
-  | ._ (get_local idx tp) := evaluator.local_at_idx idx tp -- fixme: why nat_expr here over nat?
+  | ._ (expression.get_local idx tp) := evaluator.local_at_idx idx tp -- fixme: why nat_expr here over nat?
 
-end expression
-
-namespace action
-
-def eval : action -> evaluator unit
-  | (set l e) := do v <- e.eval,
-                    l.set v
-  | (@local_def tp idx e) := do 
-    v <- e.eval,
+def action.eval : action -> evaluator unit
+  | (action.set l e) := do v <- expression.eval e,
+                    lhs.set l v
+  | (@action.local_def tp idx e) := do 
+    v <- expression.eval e,
     modify (λs, { s with locals := s.locals.insert idx (sigma.mk tp v)})
-  | (event e) := throw "event"
-  | (mk_undef l) := throw "mk_undef"
-
-end action
-
-namespace pattern
+  | (action.event e) := throw "event"
+  | (action.mk_undef l) := throw "mk_undef"
 
 -- FIXME: check pattern.context |- environment
-def eval (p : pattern) (e : environment) : evaluator unit := do
+def pattern.eval (p : pattern) (e : environment) : evaluator unit := do
   -- only machine_state is preserved across instructions
   modify (λs, { evaluator_state.empty with machine_state := s.machine_state, environment := e }),
   monad.mapm' action.eval p.actions,
   return ()
 
-end pattern
+end with_nat_env
 
 end x86
 
